aspec: msg_align_bits and related are arch independent
While the numerical value is arch dependent, the definition and symbolic value
are not. This commit factors out the symbolic computation and only unfolds the
numeric value in the architecture dependent spec.

spec/abstract/Structures_A.thy
@@ -547,6 +547,7 @@ information.
 *}
 record 'a state = abstract_state + exst :: 'a
 
+section \<open>Helper functions\<close>
 
 text {* This wrapper lifts monadic operations on the underlying machine state to
 monadic operations on the kernel state. *}
@@ -644,5 +645,56 @@ text {* The set of all caps contained in a kernel object. *}
 definition
   caps_of :: "kernel_object \<Rightarrow> cap set" where
   "caps_of kobj \<equiv> ran (cap_of kobj)"
+
+section "Cap transfers"
+
+record captransfer =
+  ct_receive_root :: cap_ref
+  ct_receive_index :: cap_ref
+  ct_receive_depth :: data
+
+definition
+  captransfer_size :: "nat" -- "in words"
+where
+  "captransfer_size \<equiv> 3"
+
+text {* A thread's IPC buffer capability must be to a page that is capable of
+containing the IPC buffer without the end of the buffer spilling into another
+page. *}
+definition cap_transfer_data_size :: nat
+where
+  "cap_transfer_data_size \<equiv> 3"
+
+definition msg_max_length :: nat
+where
+  "msg_max_length \<equiv> 120"
+
+definition msg_max_extra_caps :: nat
+where
+  "msg_max_extra_caps \<equiv> 3"
+
+definition msg_align_bits :: nat
+where
+  "msg_align_bits \<equiv>
+     word_size_bits +
+     (LEAST n. cap_transfer_data_size + msg_max_length + msg_max_extra_caps + 2 \<le> 2 ^ n)"
+
+lemma msg_align_bits':
+  "msg_align_bits = word_size_bits + 7"
+proof -
+  have "(LEAST n. (cap_transfer_data_size + msg_max_length + msg_max_extra_caps + 2) \<le> 2 ^ n) = 7"
+  proof (rule Least_equality)
+    show "(cap_transfer_data_size + msg_max_length + msg_max_extra_caps + 2)  \<le> 2 ^ 7"
+      by (simp add: cap_transfer_data_size_def msg_max_length_def msg_max_extra_caps_def)
+  next
+    fix y
+    assume "(cap_transfer_data_size + msg_max_length + msg_max_extra_caps + 2) \<le> 2 ^ y"
+    hence "(2 :: nat) ^ 7 \<le> 2 ^ y"
+      by (simp add: cap_transfer_data_size_def msg_max_length_def msg_max_extra_caps_def)
+    thus "7 \<le> y"
+      by (rule power_le_imp_le_exp [rotated], simp)
+  qed
+  thus ?thesis unfolding msg_align_bits_def by simp
+qed
 
 end
