spec/abstract/X64/ArchVSpace_A.thy
@@ -443,44 +443,6 @@ definition
   is_valid_vtable_root :: "cap \<Rightarrow> bool" where
   "is_valid_vtable_root c \<equiv> \<exists>r a. c = ArchObjectCap (PML4Cap r (Some a))"
 
-text {* A thread's IPC buffer capability must be to a page that is capable of
-containing the IPC buffer without the end of the buffer spilling into another
-page. *}
-definition
-  cap_transfer_data_size :: nat where
-  "cap_transfer_data_size \<equiv> 3"
-
-definition
-  msg_max_length :: nat where
- "msg_max_length \<equiv> 120"
-
-definition
-  msg_max_extra_caps :: nat where
- "msg_max_extra_caps \<equiv> 3"
-
-definition
-  msg_align_bits :: nat
-  where
-  "msg_align_bits \<equiv> word_size_bits + (LEAST n. (cap_transfer_data_size + msg_max_length + msg_max_extra_caps + 2) \<le> 2 ^ n)"
-
-lemma msg_align_bits:
-  "msg_align_bits = 10"
-proof -
-  have "(LEAST n. (cap_transfer_data_size + msg_max_length + msg_max_extra_caps + 2) \<le> 2 ^ n) = 7"
-  proof (rule Least_equality)
-    show "(cap_transfer_data_size + msg_max_length + msg_max_extra_caps + 2)  \<le> 2 ^ 7"
-      by (simp add: cap_transfer_data_size_def msg_max_length_def msg_max_extra_caps_def)
-  next
-    fix y
-    assume "(cap_transfer_data_size + msg_max_length + msg_max_extra_caps + 2) \<le> 2 ^ y"
-    hence "(2 :: nat) ^ 7 \<le> 2 ^ y"
-      by (simp add: cap_transfer_data_size_def msg_max_length_def msg_max_extra_caps_def)
-    thus "7 \<le> y"
-      by (rule power_le_imp_le_exp [rotated], simp)
-  qed
-  thus ?thesis unfolding msg_align_bits_def by (simp add: word_size_bits_def)
-qed
-
 definition
 check_valid_ipc_buffer :: "vspace_ref \<Rightarrow> cap \<Rightarrow> (unit,'z::state_ext) se_monad" where
 "check_valid_ipc_buffer vptr c \<equiv> case c of
@@ -530,6 +492,9 @@ definition
   prepare_thread_delete :: "obj_ref \<Rightarrow> (unit,'z::state_ext) s_monad"
 where
   "prepare_thread_delete thread_ptr \<equiv> fpu_thread_delete thread_ptr"
+
+text {* Make numeric value of @{const msg_align_bits} visible. *}
+lemmas msg_align_bits = msg_align_bits'[unfolded word_size_bits_def, simplified]
 
 end
 end
